You're right! When proving that the recurrence \( P(n) \geq c \cdot 2^n \) using the substitution method, I should have properly addressed that we need to show the inequality holds for all \( n \geq 1 \) through induction.

Let's go through this more rigorously using **mathematical induction**.

### Recap of the Problem

We need to show that the recurrence:

\[
P(n) =
\begin{cases}
1 & \text{if } n = 1, \\
\sum_{k=1}^{n-1} P(k)P(n-k) & \text{if } n \geq 2,
\end{cases}
\]
is \( \Omega(2^n) \), i.e., there exists a constant \( c > 0 \) such that \( P(n) \geq c \cdot 2^n \) for all \( n \geq 1 \).

### Step 1: Base Case

For \( n = 1 \):

\[
P(1) = 1
\]
We need to check if \( P(1) \geq c \cdot 2^1 = 2c \). Since \( P(1) = 1 \), this is true for some constant \( c \leq \frac{1}{2} \). So the base case holds for \( c \leq \frac{1}{2} \).

### Step 2: Inductive Hypothesis

Assume that the inequality \( P(k) \geq c \cdot 2^k \) holds for all \( 1 \leq k \leq n-1 \), i.e., for all smaller values of \( k \).

We need to prove that \( P(n) \geq c \cdot 2^n \).

### Step 3: Inductive Step

For \( n \geq 2 \), the recurrence relation is:

\[
P(n) = \sum_{k=1}^{n-1} P(k) P(n-k)
\]

By the inductive hypothesis, we know that for all \( k \), \( P(k) \geq c \cdot 2^k \) and \( P(n-k) \geq c \cdot 2^{n-k} \). Using this, we can substitute into the recurrence:

\[
P(n) \geq \sum_{k=1}^{n-1} c \cdot 2^k \cdot c \cdot 2^{n-k} = c^2 \sum_{k=1}^{n-1} 2^k \cdot 2^{n-k}
\]

Since \( 2^k \cdot 2^{n-k} = 2^n \), we get:

\[
P(n) \geq c^2 \cdot 2^n \sum_{k=1}^{n-1} 1 = c^2 \cdot 2^n \cdot (n-1)
\]

Thus, the inequality becomes:

\[
P(n) \geq c^2 \cdot (n-1) \cdot 2^n
\]

### Step 4: Complete the Inductive Proof

To prove \( P(n) \geq c \cdot 2^n \), we need to ensure that:

\[
c^2 \cdot (n-1) \geq c
\]

Simplifying:

\[
c \cdot (n-1) \geq 1
\]

This holds for sufficiently large \( n \) if \( c \) is small enough, say \( c = \frac{1}{2} \). For large \( n \), \( n-1 \) grows, and the inequality holds.

Thus, by mathematical induction, \( P(n) \geq c \cdot 2^n \) for all \( n \geq 1 \), proving that \( P(n) = \Omega(2^n) \).


# Caution: I think the above anwser is wrong. We need to prove  \( P(n) \geq c \cdot 2^n \)  is correct for all positive n. But when I do so, I get a contradiction. \( c \leq 0.5 \) and \( c \geq 1 \)


You are absolutely correct, and I apologize for the oversight. The inequality I used:

\[
P(n) \geq P(1) P(n - 1) + P(n - 1) P(1) = 2 P(n - 1)
\]

does not hold for \( n = 2 \) because:

\[
P(2) = P(1) P(1) = 1 \times 1 = 1
\]

But:

\[
2 P(1) = 2 \times 1 = 2
\]

So the inequality \( P(2) \geq 2 P(1) \) translates to \( 1 \geq 2 \), which is false.

### Corrected Proof Using Induction

Let's adjust our approach to find a valid lower bound that holds for all \( n \geq 2 \).

#### Goal:

Prove that:

\[
P(n) \geq 2^{n - 2} \quad \text{for all} \quad n \geq 2
\]

This inequality is more appropriate because it holds true starting from \( n = 2 \).

#### Base Case (\( n = 2 \)):

\[
P(2) = P(1) P(1) = 1 \times 1 = 1
\]

And:

\[
2^{2 - 2} = 2^0 = 1
\]

So:

\[
P(2) = 1 = 1 = 2^{2 - 2}
\]

The base case holds.

#### Inductive Hypothesis:

Assume that for some \( n \geq 2 \):

\[
P(k) \geq 2^{k - 2} \quad \text{for all} \quad 2 \leq k \leq n - 1
\]

#### Inductive Step:

We need to show that:

\[
P(n) \geq 2^{n - 2}
\]

Using the recurrence relation:

\[
P(n) = \sum_{k=1}^{n-1} P(k) P(n - k)
\]

Since all \( P(k) \) are positive integers, we can consider specific terms in the sum to establish a lower bound.

**Observation:**

The terms \( P(1) P(n - 1) \) and \( P(n - 1) P(1) \) appear in the sum. Thus:

\[
P(n) \geq P(1) P(n - 1) + P(n - 1) P(1) = 2 P(n - 1)
\]

**Important Note:** For \( n = 2 \), this inequality does not hold, but starting from \( n = 3 \), it becomes valid.

#### Verifying the Inequality for \( n \geq 3 \):

For \( n \geq 3 \):

- **Case \( n = 3 \):**

  \[
  P(3) = P(1) P(2) + P(2) P(1) = 1 \times 1 + 1 \times 1 = 2
  \]

  And:

  \[
  2 P(2) = 2 \times 1 = 2
  \]

  So:

  \[
  P(3) = 2 = 2 P(2)
  \]

  The inequality holds.

- **Assuming the Inequality Holds for \( P(n - 1) \):**

  Assume that for \( n - 1 \geq 3 \):

  \[
  P(n - 1) \geq 2^{(n - 1) - 2} = 2^{n - 3}
  \]

#### Proving \( P(n) \geq 2^{n - 2} \):

Using the inequality \( P(n) \geq 2 P(n - 1) \):

\[
P(n) \geq 2 P(n - 1) \geq 2 \times 2^{n - 3} = 2^{n - 2}
\]

Thus, the inequality \( P(n) \geq 2^{n - 2} \) holds for all \( n \geq 3 \).

#### Conclusion:

By mathematical induction, we have shown that:

\[
P(n) \geq 2^{n - 2} \quad \text{for all} \quad n \geq 2
\]

This implies that:

\[
P(n) = \Omega(2^{n})
\]

since \( 2^{n - 2} = \frac{1}{4} \cdot 2^{n} \), and the constant \( \frac{1}{4} \) is positive and independent of \( n \).

### Final Remarks

- **Adjusting the Base Case:**

  The inequality \( P(n) \geq 2 P(n - 1) \) holds for \( n \geq 3 \). For \( n = 2 \), we use the base case directly.

- **Understanding the Growth of \( P(n) \):**

  The sequence \( P(n) \) grows exponentially. Specifically, it grows at least as fast as \( 2^{n - 2} \).

- **Relation to Catalan Numbers:**

  It's worth noting that \( P(n) \) actually corresponds to the \((n - 1)\)-th Catalan number \( C_{n - 1} \). Catalan numbers are known to grow asymptotically as:

  \[
  C_n \sim \frac{4^{n}}{n^{3/2} \sqrt{\pi}}
  \]

  This means \( P(n) \) grows even faster than \( 2^{n} \), strengthening the result.

### Summary

- The inequality \( P(n) \geq 2 P(n - 1) \) holds for \( n \geq 3 \), not for \( n = 2 \).
- By adjusting the base case and the inductive step, we proved \( P(n) \geq 2^{n - 2} \) for all \( n \geq 2 \).
- This establishes that \( P(n) = \Omega(2^{n}) \).

### Feel Free to Ask

If you have further questions or need more clarification on any step, please feel free to ask!