You're absolutely right. The `COUNTING-SORT` algorithm requires that we place the elements in the output array by traversing the input array \( A \) in reverse order. Let's correct the steps and illustrate the process properly.

### Step-by-Step Illustration of COUNTING-SORT

Given the array:
\[ A = \{6, 0, 2, 0, 1, 3, 4, 6, 1, 3, 2\} \]

### Step 1: Determine the Range of the Input
The range of the input array \( A \) is from 0 to 6.

### Step 2: Initialize the Count Array
Create a count array \( C \) of size 7 (since the maximum value is 6) and initialize it to zero.

\[ C = [0, 0, 0, 0, 0, 0, 0] \]

### Step 3: Count the Occurrences
Count the occurrences of each value in the input array \( A \) and store these counts in the count array \( C \).

\[ A = \{6, 0, 2, 0, 1, 3, 4, 6, 1, 3, 2\} \]

- \( C[0] = 2 \) (since 0 appears twice)
- \( C[1] = 2 \) (since 1 appears twice)
- \( C[2] = 3 \) (since 2 appears three times)
- \( C[3] = 2 \) (since 3 appears twice)
- \( C[4] = 1 \) (since 4 appears once)
- \( C[5] = 0 \) (since 5 does not appear)
- \( C[6] = 2 \) (since 6 appears twice)

So, the count array \( C \) becomes:

\[ C = [2, 2, 3, 2, 1, 0, 2] \]

### Step 4: Modify the Count Array
Modify the count array \( C \) such that each element at each index \( i \) now contains the number of elements less than or equal to \( i \).

\[ C = [2, 4, 7, 9, 10, 10, 12] \]

### Step 5: Output Array Initialization
Create an output array \( B \) of the same size as \( A \) and initialize it to zeros.

\[ B = [0, 0, 0, 0, 0, 0, 0, 0, 0, 0, 0] \]

### Step 6: Place the Elements in the Output Array (in Reverse Order)
Place the elements from \( A \) into the output array \( B \) based on the modified count array \( C \), traversing \( A \) in reverse order.

- \( A[10] = 2 \): Place 2 in \( B[C[2] - 1] \), so \( B[6] = 2 \), and decrement \( C[2] \) to 2.
- \( A[9] = 3 \): Place 3 in \( B[C[3] - 1] \), so \( B[8] = 3 \), and decrement \( C[3] \) to 1.
- \( A[8] = 1 \): Place 1 in \( B[C[1] - 1] \), so \( B[3] = 1 \), and decrement \( C[1] \) to 1.
- \( A[7] = 6 \): Place 6 in \( B[C[6] - 1] \), so \( B[11] = 6 \), and decrement \( C[6] \) to 1.
- \( A[6] = 4 \): Place 4 in \( B[C[4] - 1] \), so \( B[9] = 4 \), and decrement \( C[4] \) to 0.
- \( A[5] = 3 \): Place 3 in \( B[C[3] - 1] \), so \( B[7] = 3 \), and decrement \( C[3] \) to 0.
- \( A[4] = 1 \): Place 1 in \( B[C[1] - 1] \), so \( B[2] = 1 \), and decrement \( C[1] \) to 0.
- \( A[3] = 0 \): Place 0 in \( B[C[0] - 1] \), so \( B[1] = 0 \), and decrement \( C[0] \) to 1.
- \( A[2] = 2 \): Place 2 in \( B[C[2] - 1] \), so \( B[5] = 2 \), and decrement \( C[2] \) to 1.
- \( A[1] = 0 \): Place 0 in \( B[C[0] - 1] \), so \( B[0] = 0 \), and decrement \( C[0] \) to 0.
- \( A[0] = 6 \): Place 6 in \( B[C[6] - 1] \), so \( B[10] = 6 \), and decrement \( C[6] \) to 0.

### Final Sorted Array
The final sorted array \( B \) is:

\[ B = [0, 0, 1, 1, 2, 2, 2, 3, 3, 4, 6, 6] \]

So, the sorted array is:

\[ \{0, 0, 1, 1, 2, 2, 2, 3, 3, 4, 6, 6\} \]